fixing up some things in CpsK2Low.

src/CpsK2Low.v
@@ -30,200 +30,200 @@ Section maps.
   Variable map_cont : Type -> Type.
   Context {FM_cont : DMap CPSK.cont map_cont}.
 
-Section monadic.
-  Import MonadNotation.
-  Local Open Scope monad_scope.
-  Local Open Scope string_scope.
+  Section monadic.
+    Import MonadNotation.
+    Local Open Scope monad_scope.
+    Local Open Scope string_scope.
 
-  Variable m : Type -> Type.
-  Context {Monad_m : Monad m}.
-  Context {Exc_m : MonadExc string m}.
-  Context {Fresh_m : MonadState positive m}.
-  Context {Freshl_m : MonadState positive m}.
-  Context {Block_m : MonadState (option (label * list var * list instr)) m}.
-  Context {Blocks_m : MonadState (alist label block) m}.
-  Context {VarMap_m : MonadReader (map_var op) m}.
-  Context {ContMap_m : MonadReader (map_cont Low.cont) m}.
+    Variable m : Type -> Type.
+    Context {Monad_m : Monad m}.
+    Context {Exc_m : MonadExc string m}.
+    Context {Fresh_m : MonadState positive m}.
+    Context {Freshl_m : MonadState positive m}.
+    Context {Block_m : MonadState (option (label * list var * list instr)) m}.
+    Context {Blocks_m : MonadState (alist label block) m}.
+    Context {VarMap_m : MonadReader (map_var op) m}.
+    Context {ContMap_m : MonadReader (map_cont Low.cont) m}.
 
-  Definition freshVar : m var :=
-    x <- modify (MS := Fresh_m) (fun x => Psucc x) ;;
-    ret (Env.Anon_v x).
-  Definition freshLbl : m label :=
-    l <- modify (MS := Freshl_m) (fun x => Psucc x) ;;
-    ret ("l"++nat2string10 (nat_of_P l))%string.
+    Definition freshVar : m var :=
+      x <- modify (MS := Fresh_m) (fun x => Psucc x) ;;
+      ret (Env.Anon_v x).
+    Definition freshLbl : m label :=
+      l <- modify (MS := Freshl_m) (fun x => Psucc x) ;;
+      ret ("l"++nat2string10 (nat_of_P l))%string.
 
-  Definition emit_tm (tm : term) : m block :=
-    block_stack <- get (MonadState := Block_m) ;;
-    match block_stack with
-      | None => raise "BUG: No current block"%string
-      | Some (l, vs, is) =>
-        put None ;;
-        let blk := {| b_args := vs ; b_insns := rev is ; b_term := tm |} in
-        ret blk
-    end.
+    Definition emit_tm (tm : term) : m block :=
+      block_stack <- get (MonadState := Block_m) ;;
+      match block_stack with
+        | None => raise "BUG: No current block"%string
+        | Some (l, vs, is) =>
+          put None ;;
+          let blk := {| b_args := vs ; b_insns := rev is ; b_term := tm |} in
+            ret blk
+      end.
 
-  Definition emit_instr (i : instr) : m unit :=
-    block_stack <- get (MonadState := Block_m) ;;
-    match block_stack with
-      | None => raise "BUG: No current block"%string
-      | Some (l, vs, is) =>
-        put (Some (l, vs, i :: is))
-    end.
+    Definition emit_instr (i : instr) : m unit :=
+      block_stack <- get (MonadState := Block_m) ;;
+      match block_stack with
+        | None => raise "BUG: No current block"%string
+        | Some (l, vs, is) =>
+          put (Some (l, vs, i :: is))
+      end.
 
-  Definition add_block (l : label) (blk : block) : m unit :=
-    modify (MS := Blocks_m) (Maps.add l blk) ;;
-    ret tt.
+    Definition add_block (l : label) (blk : block) : m unit :=
+      modify (MS := Blocks_m) (Maps.add l blk) ;;
+      ret tt.
 
-  Definition newBlock {T} (l : label) (vs : list var) (c : m T) : m T :=
-    old_blk <- get (MonadState := Block_m) ;;
-    put (Some (l, vs, nil)) ;;
-    result <- c ;;
-    put old_blk ;;
-    ret result.
+    Definition newBlock {T} (l : label) (vs : list var) (c : m T) : m T :=
+      old_blk <- get (MonadState := Block_m) ;;
+      put (Some (l, vs, nil)) ;;
+      result <- c ;;
+      put old_blk ;;
+      ret result.
 
-  Definition cont2low (c : CPSK.cont) : m Low.cont :=
-    r <- asks (MR := ContMap_m) (Maps.lookup c) ;;
-    match r with
-      | Some r => ret r
-      | None => raise ("ERROR: Unknown continuation '" ++ runShow (show c) ++ "'")
-    end.
+    Definition cont2low (c : CPSK.cont) : m Low.cont :=
+      r <- asks (MR := ContMap_m) (Maps.lookup c) ;;
+      match r with
+        | Some r => ret r
+        | None => raise ("ERROR: Unknown continuation '" ++ runShow (show c) ++ "'")
+      end.
 
-  Definition withNewConts (ks : list (CPSK.cont * label)) : forall {T}, m T -> m T :=
-    @local _ _ ContMap_m (fold_left (fun acc x => Maps.add (map := map_cont) (fst x) (inr (snd x)) acc) ks).
+    Definition withNewConts (ks : list (CPSK.cont * label)) : forall {T}, m T -> m T :=
+      @local _ _ ContMap_m (fold_left (fun acc x => Maps.add (map := map_cont) (fst x) (inr (snd x)) acc) ks).
 
-  Definition withNewVars (vo : list (var * op)) : forall {T}, m T -> m T :=
-    @local _ _ VarMap_m (fold_left (fun acc x => Maps.add (fst x) (snd x) acc) vo).
+    Definition withNewVars (vo : list (var * op)) : forall {T}, m T -> m T :=
+      @local _ _ VarMap_m (fold_left (fun acc x => Maps.add (fst x) (snd x) acc) vo).
 
-  Definition withNewVar (v : var) (o : op) : forall {T}, m T -> m T :=
-    @withNewVars ((v,o) :: nil).
-  
-  Definition inFreshLbl {T} (vs:list var) (k:m T) : m (label * T) :=
-    l <- freshLbl ;;
-    result <- newBlock l vs k ;;
-    ret (l, result).
+    Definition withNewVar (v : var) (o : op) : forall {T}, m T -> m T :=
+      @withNewVars ((v,o) :: nil).
+    
+    Definition inFreshLbl {T} (vs:list var) (k:m T) : m (label * T) :=
+      l <- freshLbl ;;
+      result <- newBlock l vs k ;;
+      ret (l, result).
 
-  Definition opgen (o:op) : m op :=
-    match o with 
-      | Var_o v => 
-        x <- asks (Maps.lookup v) ;;
-        match x with
-          | None => raise ("ERROR: Unknown variable '" ++ runShow (show v) ++ "'")
-          | Some v => ret v
-        end
-      | Con_o c => ret (Con_o c)
-      | Int_o z => ret (Int_o z)
-    end.
+    Definition opgen (o:op) : m op :=
+      match o with 
+        | Var_o v => 
+          x <- asks (Maps.lookup v) ;;
+          match x with
+            | None => raise ("ERROR: Unknown variable '" ++ runShow (show v) ++ "'")
+            | Some v => ret v
+          end
+        | Con_o c => ret (Con_o c)
+        | Int_o z => ret (Int_o z)
+      end.
 
-  Definition gen_lbl_args (e:exp) : m (list var) :=
-    let vs := free_vars_exp (s := list (var + cont)) e in
-    let vs := filter (fun x => match x with
-                                 | inl _ => true
-                                 | inr _ => false
-                               end) vs in
-    mapM (fun x => match x with
-                     | inl x => ret x
-                     | inr _ => raise "BUG: found continuation after filter"%string
-                   end) vs.
+    Definition gen_lbl_args (e:exp) : m (list var) :=
+      let vs := free_vars_exp (s := list (var + cont)) e in
+        let vs := filter (fun x => match x with
+                                     | inl _ => true
+                                     | inr _ => false
+                                   end) vs in
+        mapM (fun x => match x with
+                         | inl x => ret x
+                         | inr _ => raise "BUG: found continuation after filter"%string
+                       end) vs.
 
-  Fixpoint list_repeat {A} (n:nat) (a:A) : list A :=
-    match n with
-      | O => nil
-      | S n => a :: list_repeat n a
-    end.
+    Fixpoint list_repeat {A} (n:nat) (a:A) : list A :=
+      match n with
+        | O => nil
+        | S n => a :: list_repeat n a
+      end.
 
-  Definition decl2low (d:decl) {T} (c : m T) : m T :=
-    match d with
-      | Op_d x o => 
+    Definition decl2low (d:decl) {T} (c : m T) : m T :=
+      match d with
+        | Op_d x o => 
         withNewVar x o c
-      | Prim_d x p os =>
-        vs <- mapM opgen os ;;
-        match p with
-          | CpsCommon.Eq_p => 
-            emit_instr (Primop_i x Eq_p vs)
-          | CpsCommon.Neq_p =>
-            emit_instr (Primop_i x Neq_p vs)
-          | CpsCommon.Lt_p =>
-            emit_instr (Primop_i x Lt_p vs)
-          | CpsCommon.Lte_p =>
-            emit_instr (Primop_i x Lte_p vs)
-          | CpsCommon.Ptr_p =>
-            emit_instr (Primop_i x Ptr_p vs)
-          | CpsCommon.Plus_p => 
-            emit_instr (Primop_i x Plus_p vs)
-          | CpsCommon.Minus_p => 
-            emit_instr (Primop_i x Minus_p vs)
-          | CpsCommon.Times_p => 
-            emit_instr (Primop_i x Times_p vs)
-          | CpsCommon.MkTuple_p => 
-            mtyp <- mapM (fun v => x <- freshVar ;; ret (x, Int_t, v)) vs ;;
-            emit_instr (Malloc_i (map (fun x => let '(x, t, v) := x in (x, t)) mtyp)) ;;
-            dummy <- mapM (fun x => let '(x, t, v) := x in
-              emit_instr (Store_i t v 0 (Var_o x))) mtyp ;;
-            ret tt
-          | CpsCommon.Proj_p => 
-            match vs with
-              | CpsCommon.Int_o idx :: v :: nil => 
-                (** TODO: Why do we require Int_o and Var_o here? **)
+        | Prim_d x p os =>
+          vs <- mapM opgen os ;;
+          match p with
+            | CpsCommon.Eq_p => 
+              emit_instr (Primop_i x Eq_p vs)
+            | CpsCommon.Neq_p =>
+              emit_instr (Primop_i x Neq_p vs)
+            | CpsCommon.Lt_p =>
+              emit_instr (Primop_i x Lt_p vs)
+            | CpsCommon.Lte_p =>
+              emit_instr (Primop_i x Lte_p vs)
+            | CpsCommon.Ptr_p =>
+              emit_instr (Primop_i x Ptr_p vs)
+            | CpsCommon.Plus_p => 
+              emit_instr (Primop_i x Plus_p vs)
+            | CpsCommon.Minus_p => 
+              emit_instr (Primop_i x Minus_p vs)
+            | CpsCommon.Times_p => 
+              emit_instr (Primop_i x Times_p vs)
+            | CpsCommon.MkTuple_p => 
+              mtyp <- mapM (fun v => x <- freshVar ;; ret (x, Int_t, v)) vs ;;
+              emit_instr (Malloc_i (map (fun x => let '(x, t, v) := x in (x, t)) mtyp)) ;;
+              dummy <- mapM (fun x => let '(x, t, v) := x in
+                emit_instr (Store_i t v 0 (Var_o x))) mtyp ;;
+              ret tt
+            | CpsCommon.Proj_p => 
+              match vs with
+                | CpsCommon.Int_o idx :: v :: nil => 
+                (** TODO: Why do we require Int_o here? **)
                 (** TODO: [length vs] is wrong here. **)
-                emit_instr (Load_i x (Struct_t (list_repeat (length vs) Int_t)) idx v)
-              | _ => raise ("ERROR: Proj_p requires exactly 2 arguments"%string)
-            end
-        end ;;
+                  emit_instr (Load_i x (Struct_t (list_repeat (length vs) Int_t)) idx v)
+                | _ => raise ("ERROR: Proj_p requires exactly 2 arguments"%string)
+              end
+          end ;;
         withNewVar x (Var_o x) c
-      | Fn_d _ _ _ _ => raise ("ERROR: Function found in closure converted body"%string) 
-      | Bind_d x _ mop _ => 
-        match mop return m unit with end ;;
+        | Fn_d _ _ _ _ => raise ("ERROR: Function found in closure converted body"%string) 
+        | Bind_d x _ mop _ => 
+          match mop return m unit with end ;;
         withNewVar x (Var_o x) c
-    end.
-  
-  Fixpoint cpsk2low' (e:exp) : m block :=
-    match e with
-      | App_e o ks os => 
-        v <- opgen o ;;
-        vs <- mapM opgen os ;;
-        x <- freshVar ;;
-        ks <- mapM cont2low ks ;;
-        emit_tm (Call_tm x v vs ks)
-      | Let_e d e => 
-        decl2low d (cpsk2low' e)
-      | Letrec_e ds e => 
-        binders <- mapM (fun d =>
-          match d with
-            | Prim_d x _ _ 
-            | Fn_d x _ _ _ 
-            | Bind_d x _ _ _
-            | Op_d x _ => ret (x, Var_o x)
-          end) ds ;;
-        let _ : list (var * op) := binders in
+      end.
+    
+    Fixpoint cpsk2low' (e:exp) : m block :=
+      match e with
+        | App_e o ks os => 
+          v <- opgen o ;;
+          vs <- mapM opgen os ;;
+          x <- freshVar ;;
+          ks <- mapM cont2low ks ;;
+          emit_tm (Call_tm x v vs ks)
+        | Let_e d e => 
+          decl2low d (cpsk2low' e)
+        | Letrec_e ds e => 
+          binders <- mapM (fun d =>
+            match d with
+              | Prim_d x _ _ 
+              | Fn_d x _ _ _ 
+              | Bind_d x _ _ _
+              | Op_d x _ => ret (x, Var_o x)
+            end) ds ;;
+          let _ : list (var * op) := binders in
         withNewVars binders
           (iterM (fun x => decl2low x (ret tt)) ds ;;
-           cpsk2low' e)
-      | Switch_e o arms e =>
-        v <- opgen o ;;
-        arms <- mapM (fun pat =>
-          let '(p,e) := pat in
-            lbl_blk <- inFreshLbl nil (cpsk2low' e) ;;
-            add_block (fst lbl_blk) (snd lbl_blk) ;;
-            ret (p, fst lbl_blk, map (fun x => Var_o x) nil)) arms ;;
-        defLbl <- match e with
-                    | None => ret None
-                    | Some e => 
-                      lbl_blk <- inFreshLbl nil (cpsk2low' e) ;;
-                      add_block (fst lbl_blk) (snd lbl_blk) ;;
-                      ret (Some (fst lbl_blk, nil))
-                  end ;;
-        emit_tm (Switch_tm v arms defLbl)
-      | Halt_e o _ => 
-        v <- opgen o ;;
-        emit_tm (Halt_tm v)
-      | AppK_e k os => 
-        k <- cont2low k ;;
-        vs <- mapM opgen os ;;
-        emit_tm (Cont_tm k vs)
-      | LetK_e cves e => 
-        lbls <- mapM (fun x => let '(k, vs, e) := x in 
-          l <- freshLbl ;;
-          ret (k, l)) cves ;;
+            cpsk2low' e)
+        | Switch_e o arms e =>
+          v <- opgen o ;;
+          arms <- mapM (fun pat =>
+            let '(p,e) := pat in
+              lbl_blk <- inFreshLbl nil (cpsk2low' e) ;;
+              add_block (fst lbl_blk) (snd lbl_blk) ;;
+              ret (p, fst lbl_blk, map (fun x => Var_o x) nil)) arms ;;
+          defLbl <- match e with
+                      | None => ret None
+                      | Some e => 
+                        lbl_blk <- inFreshLbl nil (cpsk2low' e) ;;
+                        add_block (fst lbl_blk) (snd lbl_blk) ;;
+                        ret (Some (fst lbl_blk, nil))
+                    end ;;
+          emit_tm (Switch_tm v arms defLbl)
+        | Halt_e o _ => 
+          v <- opgen o ;;
+          emit_tm (Halt_tm v)
+        | AppK_e k os => 
+          k <- cont2low k ;;
+          vs <- mapM opgen os ;;
+          emit_tm (Cont_tm k vs)
+        | LetK_e cves e => 
+          lbls <- mapM (fun x => let '(k, vs, e) := x in 
+            l <- freshLbl ;;
+            ret (k, l)) cves ;;
         withNewConts
           (map (fun x => let '(k, l) := x in (k, l)) lbls)
           ((iterM (fun x => let '(k, vs, e) := x in 
@@ -234,16 +234,18 @@ Section monadic.
                 add_block l blk
               | inl _ => raise "??: local cont references cont parameter"%string
             end) cves) ;;
-            cpsk2low' e)
-    end.
+          cpsk2low' e)
+      end.
 
-  Fixpoint tl_cpsk2low (e:exp) : m (label * block) :=
-    l <- freshLbl ;;
-    blk <- cpsk2low' e ;;
-    add_block l blk ;;
-    ret (l, blk).
+    Fixpoint tl_cpsk2low (e:exp) : m (label * block) :=
+      l <- freshLbl ;;
+      blk <- cpsk2low' e ;;
+      add_block l blk ;;
+      ret (l, blk).
 
-End monadic.
+  End monadic.
+
+End maps.
 
 Section monadic2.
   Import MonadNotation.
@@ -253,13 +255,6 @@ Section monadic2.
   Context {Monad_m : Monad m}.
   Context {Exc_m : MonadExc string m}.
 
-(*
-Context {Monad_m : Monad m}.
-  Context {Exc_m : MonadExc string m}.
-  Context {VarMap_m : MonadReader (map_var op) m}.
-  Context {ContMap_m : MonadReader (map_cont Low.cont) m}.
-*)
-
   Record StateData : Type :=
   { freshVar_p : positive
   ; freshLabel_p : positive
@@ -267,8 +262,8 @@ Context {Monad_m : Monad m}.
   ; allBlocks : alist label block
   }.
   Record ReaderData : Type :=
-  { varMap : map_var op
-  ; contMap : map_cont Low.cont
+  { varMap : alist var op
+  ; contMap : alist CPSK.cont Low.cont
   }.
 
   Definition MonadState_StateData_freshVar m (M : Monad m) : MonadState _ (stateT StateData m) :=
@@ -293,11 +288,15 @@ Context {Monad_m : Monad m}.
 
   Instance MonadReader_ReaderData_contMap m (M : Monad m) : MonadReader _ (readerT ReaderData m) :=
     ReaderProd contMap (fun x d => {| varMap := d.(varMap) ; contMap := x |}).
+  About tl_cpsk2low.
 
-  Arguments tl_cpsk2low {m Mon MExc MSvar MSlbl _ _ _ _} (e) : rename.
+  Arguments tl_cpsk2low {_ _ _ _ m Mon MExc MSvar MSlbl _ _ _ _} (e) : rename.
 
-  Definition tl_decl2low (name : var) (ks : list cont) (args : list var) (e : CPSK.exp) : m Low.function :=
-    let c := tl_cpsk2low (m := stateT StateData (readerT ReaderData m))
+  Definition tl_decl2low (name : var) (ks : list CPSK.cont) (args : list var) (e : CPSK.exp) : m Low.function :=
+    let c := tl_cpsk2low 
+      (map_var := alist var) (FM_var := DMap_alist RelDec_var_eq)
+      (map_cont := alist CPSK.cont) (FM_cont := DMap_alist CPSK.RelDec_cont_eq)
+      (m := stateT StateData (readerT ReaderData m))
       (MSvar := MonadState_StateData_freshVar _ _)
       (MSlbl := MonadState_StateData_freshLabel_p _ _)
       e in
@@ -321,26 +320,13 @@ Context {Monad_m : Monad m}.
          ; f_body := state.(allBlocks)
          ; f_entry := entry_label |}.
 
-  Definition tl_cpsk2low' (fs : list decl) (e : exp) : m Low.program.
-  refine (
+  Definition cpsk2low (fs : list CPSK.decl) (e : CPSK.exp) : m Low.program :=
     fs <- mapM (fun d => 
       match d with
-        | Fn_d f ks args e => tl_decl2low f ks args e
+        | CPSK.Fn_d f ks args e => tl_decl2low f ks args e
         | _ => raise ("Decl other than function found in top-lvl")%string
       end) fs ;;
     entry <- tl_decl2low (Named_v "main"%string None) nil nil e ;;
-    ret {| p_topdecl := entry::fs; p_entry := (Named_v "main"%string None) |}
-    ).
-  Defined.
+    ret {| p_topdecl := entry::fs; p_entry := (Named_v "main"%string None) |}.
+
 End monadic2.
-
-End maps.
-
-Definition cpsk2low (fs : list CPSK.decl) (e : CPSK.exp) : string + Low.program.
-refine (
-  match tl_cpsk2low' _ _ _ fs e with
-    | inl ex => inl ex
-    | inr prog => inr prog
-  end
-).
-Defined.
